\documentclass[tbtags]{cheatsheet}
\usepackage{amsmath}
\usepackage{esdiff}
\setlength{\mathindent}{0pt}

\begin{document}
	\section{Miscellanea}	
		\begin{gather*}
			\left|\frac{\partial(x,y,z)}{\partial(r,\theta,\phi)}\right| = r^2 \sin \theta \\
			\left| \frac{\partial(x,y)}{\partial(r,\theta)} \right| = \left| \frac{\partial(x,y,z)}{\partial(r,\phi,z)} \right| = r\\
			\int \frac{\mathrm{d}x}{x} = \ln|x| + C\\
			\sin\theta \xrightarrow{\diff{}{\theta}} \cos\theta \rightarrow -\sin\theta\\
			%\xrightleftharpoons[d]{test}
		\end{gather*}
	\subsection{Trigonometry}
		\begin{gather*}
			\frac{\sin a}{A} = \frac{\sin b}{B} = \frac{\sin c}{C}	\tag{law of sines}\\
			C = \sqrt{A^2 + B^2 - 2AB\cos(c)}	\tag{law of cosines}
		\end{gather*}
		\subsubsection{Identities}
			\begin{gather*}
				\sin^2\theta + \cos^2\theta = 1\\
				\sin(\theta \pm \frac{\pi}{2}) = \pm\cos\theta\\
				\begin{split}
					\sin(\alpha \pm \beta) &= \sin\alpha\cos\beta\\
					 &\pm \cos\alpha\sin\beta
				\end{split}\\
				\begin{split}
					\cos(\alpha \pm \beta) &= \cos\alpha\cos\beta \\
					&\mp \sin\alpha\sin\beta
				\end{split}\\
				\sin^2 \theta = \frac{1-\cos(2\theta)}{2}\\
				\cos^2 \theta = \frac{1+\cos(2\theta)}{2}\\
				\sin(2\theta) = 2\sin\theta\cos\theta\\
				\begin{split}
					\cos(2\theta) &= \cos^2\theta - \sin^2\theta\\
					&= 2\cos^2\theta - 1\\
					&= 1 - 2\sin^2\theta
				\end{split}
			\end{gather*}
	\subsection{Derivatives}
		\begin{gather*}
			\diff{(uv)}{x} = u'v + uv'	\\
			\diff{(u/v)}{x} = \frac{u'v - uv'}{v^2}	\\
			\diff{( u(v) )}{x} = u'(v)v'
		\end{gather*}
	\subsection{Kinematics}
		\begin{gather*}
			\vec v(t) = \vec v_0 + \vec at 	\tag{velocity}\\
			\vec \omega(t) = \vec\omega_0 + \vec\alpha t	\tag{rot. form}\\
			\vec x(t) = \vec x_0 + \vec vt + \frac{1}{2}\vec a t^2	\tag{displacement}\\
			\vec\theta(t) = \vec\theta_0 + \vec\omega t + \frac{1}{2}\alpha t^2	\tag{rot. form}\\
			v_f = \sqrt{{v_i}^2 + 2a\Delta x}	\tag{$v_f$}
		\end{gather*}

	\section{Momentum}
	\begin{gather*}
		\vec p = m\vec v	\tag{momentum}\\
		\vec\ell = I\vec\omega = \vec r \times \vec p	\tag{rot. form}\\
		\dot{\vec P} = \vec F_\mathrm{ext} \tag{3rd law}\\
		\dot{\vec\ell} = \vec\tau = I\vec\alpha= \vec r \times \vec F	\tag{rot. form}\\
		\begin{split}
				\Delta\vec P &= \vec P_f - \vec P_i = \vec J	\\
			&= \int \vec F \mathrm{d}t	\\
			&= \vec F_\text{avg}\Delta t
		\end{split}\tag{impulse}\\
	\end{gather*}
		\subsection{Total Angular Momentum}
		\begin{align*}
			\vec L &= \sum_{i=1}^{N} \vec\ell_i	\\
			&= \vec R_\text{CM} \times \vec P_\text{CM}	\tag{$\vec L_\text{orb}$ of CM about axis}\\
			&+ \sum_{i=1}^{N} r_i' \times \vec p_i\,'		\tag{$\vec L_\text{spin}$ of body about CM}
		\end{align*}
		\subsection{Collisions}
			An \emph{elastic} collision conserves kinetic energy.
			\[
				m_1\vec v_1 + m_2\vec v_2 = m_1\vec v_1\,' + m_2\vec v_2\,'
			\]
			An \emph{inelastic} collision does not.
			\[
				m_1\vec v_1 + m_2\vec v_2 = m\vec v\,'
			\]
	\section{Changing Mass}
		\subsection{Rockets}
			\begin{gather*}
				\vec F_\mathrm{th} = -\dot{m}\vec v_\mathrm{ex}		\tag{thrust}\\
				\vec v(t) = \vec v_0 + \vec v_\mathrm{ex}\ln\left( \frac{m_0}{m(t)} \right)	\tag{$\Delta V$}
			\end{gather*}
	\section{Center of Mass}
	\begin{gather*}
		\vec R = \frac{1}{M}\sum_{i=1}^N m_i \vec r_i	\tag{CM summation}\raisetag{-10pt}\\
		M = \int \rho \mathrm{d}V	\tag{total mass}\\
		\vec R =  \frac{1}{M}  \int \vec r \mathrm{d}m \tag{CM integral}\raisetag{-6pt}\\
	\intertext{$\mathrm{d}m$ can usually be rewritten in terms of $\mathrm{d}V$}
		\vec R = \frac{1}{M} \int \vec r \rho(\vec r) \mathrm{d}V
	\end{gather*}
	Look for symmetries by which you can substitute $\vec R$ and $\vec r$ for scalars.

	\section{Moment of Inertia}
	\begin{gather*}
		\sum_{i=1}^{N} = m_i r^2_\perp \tag{summation}\\
		I = \int r^2_\perp \mathrm{d}m	\tag{integral}
	\end{gather*}
		\subsection{Parallel Axis Theorem}
			\[ I = I_\mathrm{CM} + Md^2 \]
			where $I \parallel I_\mathrm{CM}$ and $d$ is the distance between $I$ \& $I_\mathrm{CM}$

		\subsection{Perpendicular Axis Theorem}
			For \emph{planar lamina} (flat, plate-like objects)
			\[ I_z = I_x + I_y \]


	\section{Work \& Energy}
		\begin{gather*}
			\begin{split}
			W &= \int_C \vec{F} \cdot \mathrm{d}\vec{r}	\\
			&= \int_{a}^b \vec{F}\left( \vec{r}(t) \right) \cdot \vec{r}\,'(t)\mathrm{d}t \\
			&= \int_{x,y} \left\langle F_x, F_y \right\rangle \cdot \left\langle \mathrm{d}x, \mathrm{d}y \right\rangle
			\end{split}\tag{work integral}\\
			W = \Delta T	\tag{Work-Energy Theorem}\\
			\vec F = -\nabla U	\tag{potential from force}
		\end{gather*}

%		\subsection{Line Integrals}
%			\begin{gather*}
%				\begin{split}
%					&\int_{C} f\left( \vec{r}(t) \right) \mathrm{d}s \\
%					&=\int_{a}^b f\left( \vec{r}(t) \right) \left| \vec{r}\,'(t) \right| \mathrm{d}t
%				\end{split}\tag{scalar}\\
%			\end{gather*}

		\subsection{Conservative Forces}
			A \emph{conservative force} is one with a corresponding potential energy. This means:
			\begin{itemize}
				\item the force depends \emph{only} on position
				\item the work done by that force is the same for \emph{any} path $\implies \nabla \times \vec F = 0$
			\end{itemize}

	\section{Lagrangian Mechanics}
			\begin{gather*}
				\mathcal{L} = T - U	\tag{Lagrangian}\\
				\diff{}{t} \underbrace{\diffp{\mathcal{L}}{{\dot{q}_i}}}_\text{gnr. $p$} =  \overbrace{\diffp{\mathcal{L}}{{q_i}}}^\text{gnr. $F$}	\tag{$\mathcal{L}$ eqn.}
			\end{gather*}
			where 
			

\end{document}